initial commit

Earley.thy
@@ -81,7 +81,7 @@ lemma slice_shift:
   unfolding slice_drop_take by (simp add: drop_take)
 
 
-section \<open>Additional Derivation Lemmas\<close>
+section \<open>Derivation Lemmas\<close>
 
 lemma Derives1_prepend:
   assumes "Derives1 cfg u i r v"
@@ -212,7 +212,7 @@ qed
 
 section \<open>Earley recognizer\<close>
 
-subsection \<open>Earley items\<close>
+subsection \<open>Earley Items\<close>
 
 definition rule_head :: "'a rule \<Rightarrow> 'a" where
   "rule_head = fst"
@@ -227,8 +227,6 @@ datatype 'a item =
     (item_origin : nat)
     (item_end : nat)
 
-type_synonym 'a items = "'a item set"
-
 definition item_rule_head :: "'a item \<Rightarrow> 'a" where
   "item_rule_head x = rule_head (item_rule x)"
 
@@ -241,28 +239,42 @@ definition item_\<alpha> :: "'a item \<Rightarrow> 'a sentence" where
 definition item_\<beta> :: "'a item \<Rightarrow> 'a sentence" where 
   "item_\<beta> x = drop (item_dot x) (item_rule_body x)"
 
-definition init_item :: "'a rule \<Rightarrow> nat \<Rightarrow> 'a item" where
-  "init_item r k = Item r 0 k k"
-
 definition is_complete :: "'a item \<Rightarrow> bool" where
   "is_complete x = (item_dot x \<ge> length (item_rule_body x))"
 
 definition next_symbol :: "'a item \<Rightarrow> 'a option" where
-  "next_symbol x = (if is_complete x then None else Some ((item_rule_body x) ! (item_dot x)))"
-
-definition is_opening :: "'a item \<Rightarrow> bool" where
-  "is_opening x = (item_dot x = 0)"
-
-definition prev_symbol :: "'a item \<Rightarrow> 'a option" where
-  "prev_symbol x = (if is_opening x then None else Some ((item_rule_body x) ! (item_dot x - 1)))"
-
-definition inc_item :: "'a item \<Rightarrow> nat \<Rightarrow> 'a item" where
-  "inc_item x k = Item (item_rule x) (item_dot x + 1) (item_origin x) k"
+  "next_symbol x = (if is_complete x then None else Some (item_rule_body x ! item_dot x))"
 
 lemmas item_defs = item_rule_head_def item_rule_body_def item_\<alpha>_def item_\<beta>_def rule_head_def rule_body_def
 
-definition bin :: "'a items \<Rightarrow> nat \<Rightarrow> 'a items" where
-  "bin I k = { x . x \<in> I \<and> item_end x = k }"
+definition is_finished :: "'a cfg \<Rightarrow> 'a sentence \<Rightarrow> 'a item \<Rightarrow> bool" where
+  "is_finished cfg inp x \<equiv>
+    item_rule_head x = \<SS> cfg \<and>
+    item_origin x = 0 \<and>
+    item_end x = length inp \<and> 
+    is_complete x"
+
+definition earley_recognized :: "'a item set \<Rightarrow> 'a cfg \<Rightarrow> 'a sentence \<Rightarrow> bool" where
+  "earley_recognized I cfg inp = (\<exists>x \<in> I. is_finished cfg inp x)"
+
+inductive_set Earley :: "'a cfg \<Rightarrow> 'a sentence \<Rightarrow> 'a item set"
+  for \<G> :: "'a cfg" and \<omega> :: "'a sentence" where
+  Init: "r \<in> set (\<RR> \<G>) \<Longrightarrow> fst r = \<SS> \<G>
+    \<Longrightarrow> Item r 0 0 0 \<in> Earley \<G> \<omega>"
+| Scan: "x = Item r b i j \<Longrightarrow> x \<in> Earley \<G> \<omega> \<Longrightarrow>
+    \<omega>!j = a \<Longrightarrow> j < length \<omega> \<Longrightarrow> next_symbol x = Some a \<Longrightarrow>
+      Item r (b + 1) i (j + 1) \<in> Earley \<G> \<omega>"
+| Predict: "x = Item r b i j \<Longrightarrow> x \<in> Earley \<G> \<omega> \<Longrightarrow>
+    r' \<in> set (\<RR> \<G>) \<Longrightarrow> next_symbol x = Some (rule_head r') \<Longrightarrow>
+      Item r' 0 j j \<in> Earley \<G> \<omega>"
+| Complete: "x = Item r\<^sub>x b\<^sub>x i j \<Longrightarrow> x \<in> Earley \<G> \<omega> \<Longrightarrow> y = Item r\<^sub>y b\<^sub>y j k \<Longrightarrow> y \<in> Earley \<G> \<omega> \<Longrightarrow>
+    is_complete y \<Longrightarrow> next_symbol x = Some (item_rule_head y) \<Longrightarrow>
+      Item r\<^sub>x (b\<^sub>x + 1) i k \<in> Earley \<G> \<omega>"
+
+
+find_theorems Earley
+
+subsection \<open>Well-formedness\<close>
 
 definition wf_item :: "'a cfg \<Rightarrow> 'a sentence => 'a item \<Rightarrow> bool" where 
   "wf_item cfg inp x = (
@@ -271,650 +283,158 @@ definition wf_item :: "'a cfg \<Rightarrow> 'a sentence => 'a item \<Rightarrow>
     item_origin x \<le> item_end x \<and> 
     item_end x \<le> length inp)"
 
-definition wf_items :: "'a cfg \<Rightarrow> 'a sentence \<Rightarrow> 'a items \<Rightarrow> bool" where
-  "wf_items cfg inp I = (\<forall>x \<in> I. wf_item cfg inp x)"
-
-
-subsection \<open>Epsilon Productions\<close>
-
-definition \<epsilon>_free :: "'a cfg \<Rightarrow> bool" where
-  "\<epsilon>_free cfg \<longleftrightarrow> (\<forall>r \<in> set (\<RR> cfg). rule_body r \<noteq> [])"
-
-lemma \<epsilon>_free_impl_non_empty_sentence_deriv:
-  "\<epsilon>_free cfg \<Longrightarrow> a \<noteq> [] \<Longrightarrow> \<not> Derivation cfg a D []"
-proof (induction "length D" arbitrary: a D rule: nat_less_induct)
-  case 1
-  show ?case
-  proof (rule ccontr)
-    assume assm: "\<not> \<not> Derivation cfg a D []"
-    show False
-    proof (cases "D = []")
-      case True
-      then show ?thesis
-        using "1.prems"(2) assm by auto
-    next
-      case False
-      then obtain d D' \<alpha> where *:
-        "D = d # D'" "Derives1 cfg a (fst d) (snd d) \<alpha>" "Derivation cfg \<alpha> D' []" "snd d \<in> set (\<RR> cfg)"
-        using list.exhaust assm Derives1_def by (metis Derivation.simps(2))
-      show ?thesis
-      proof cases
-        assume "\<alpha> = []"
-        thus ?thesis
-          using *(2,4) Derives1_split \<epsilon>_free_def rule_body_def "1.prems"(1) by (metis append_is_Nil_conv)
-      next
-        assume "\<not> \<alpha> = []"
-        thus ?thesis
-          using *(1,3) "1.hyps" "1.prems"(1) by auto
-      qed
-    qed
-  qed
-qed
-
-lemma \<epsilon>_free_impl_non_empty_deriv:
-  "\<epsilon>_free cfg \<Longrightarrow> \<forall>N \<in> set (\<NN> cfg). \<not> derives cfg [N] []"
-  using \<epsilon>_free_impl_non_empty_sentence_deriv derives_implies_Derivation by (metis not_Cons_self2)
-
-lemma nonempty_deriv_impl_\<epsilon>_free:
-  assumes "\<forall>N \<in> set (\<NN> cfg). \<not> derives cfg [N] []" "\<forall>(N, \<alpha>) \<in> set (\<RR> cfg). N \<in> set (\<NN> cfg)"
-  shows "\<epsilon>_free cfg"
-proof (rule ccontr)
-  assume "\<not> \<epsilon>_free cfg"
-  then obtain N \<alpha> where *: "(N, \<alpha>) \<in> set (\<RR> cfg)" "rule_body (N, \<alpha>) = []"
-    unfolding \<epsilon>_free_def by auto
-  hence "derives1 cfg [N] []"
-    unfolding derives1_def rule_body_def by auto
-  hence "derives cfg [N] []"
-    by auto
-  moreover have "N \<in> set (\<NN> cfg)"
-    using *(1) assms(2) by blast
-  ultimately show False
-    using assms(1) by blast
-qed
-
-lemma nonempty_deriv_iff_\<epsilon>_free:
-  assumes "\<forall>(N, \<alpha>) \<in> set (\<RR> cfg). N \<in> set (\<NN> cfg)"
-  shows "(\<forall>N \<in> set (\<NN> cfg). \<not> derives cfg [N] []) \<longleftrightarrow> \<epsilon>_free cfg"
-  using \<epsilon>_free_impl_non_empty_deriv nonempty_deriv_impl_\<epsilon>_free[OF _ assms] by blast
-
-
-subsection \<open>Earley algorithm\<close>
-
-definition Init :: "'a cfg \<Rightarrow> 'a items" where
-  "Init cfg = { init_item r 0 | r. r \<in> set (\<RR> cfg) \<and> fst r = (\<SS> cfg) }"
-
-definition Scan :: "nat \<Rightarrow> 'a sentence \<Rightarrow> 'a items \<Rightarrow> 'a items" where
-  "Scan k inp I = 
-    { inc_item x (k+1) | x a.
-        x \<in> bin I k \<and>
-        inp!k = a \<and>
-        k < length inp \<and>
-        next_symbol x = Some a }"
-
-definition Predict :: "nat \<Rightarrow> 'a cfg \<Rightarrow> 'a items \<Rightarrow> 'a items" where
-  "Predict k cfg I =
-    { init_item r k | r x.
-        r \<in> set (\<RR> cfg) \<and>
-        x \<in> bin I k \<and>
-        next_symbol x = Some (rule_head r) }"
-
-definition Complete :: "nat \<Rightarrow> 'a items \<Rightarrow> 'a items" where
-  "Complete k I =
-    { inc_item x k | x y.
-        x \<in> bin I (item_origin y) \<and>
-        y \<in> bin I k \<and>
-        is_complete y \<and>
-        next_symbol x = Some (item_rule_head y) }"
-
-definition \<pi>_step :: "nat \<Rightarrow> 'a cfg \<Rightarrow> 'a sentence \<Rightarrow> 'a items \<Rightarrow> 'a items" where
-  "\<pi>_step k cfg inp I = I \<union> Scan k inp I \<union> Complete k I \<union> Predict k cfg I"
-
-definition \<pi> :: "nat \<Rightarrow> 'a cfg \<Rightarrow> 'a sentence \<Rightarrow> 'a items \<Rightarrow> 'a items" where
-  "\<pi> k cfg inp I = limit (\<pi>_step k cfg inp) I"
-
-fun \<I> :: "nat \<Rightarrow> 'a cfg \<Rightarrow> 'a sentence \<Rightarrow> 'a items" where
-  "\<I> 0 cfg inp = \<pi> 0 cfg inp (Init cfg)"
-| "\<I> (Suc n) cfg inp = \<pi> (Suc n) cfg inp (\<I> n cfg inp)"
-
-definition \<II> :: "'a cfg \<Rightarrow> 'a sentence \<Rightarrow> 'a items" where
-  "\<II> cfg inp = \<I> (length inp) cfg inp"
-
-definition is_finished :: "'a cfg \<Rightarrow> 'a sentence \<Rightarrow> 'a item \<Rightarrow> bool" where
-  "is_finished cfg inp x \<longleftrightarrow> (
-    item_rule_head x = \<SS> cfg \<and>
-    item_origin x = 0 \<and>
-    item_end x = length inp \<and> 
-    is_complete x)"
-
-definition earley_recognized :: "'a items \<Rightarrow> 'a cfg \<Rightarrow> 'a sentence \<Rightarrow> bool" where
-  "earley_recognized I cfg inp = (\<exists>x \<in> I. is_finished cfg inp x)"
-
-
-subsection \<open>Wellformedness\<close>
-
-lemma wf_items_Un:
-  "wf_items cfg inp I \<Longrightarrow> wf_items cfg inp J \<Longrightarrow> wf_items cfg inp (I \<union> J)"
-  unfolding wf_items_def by blast
-
-lemmas wf_defs = wf_item_def wf_items_def
-
 lemma wf_Init:
-  "x \<in> Init cfg \<Longrightarrow> wf_item cfg inp x"
-  unfolding Init_def wf_item_def init_item_def by auto
+  assumes "r \<in> set (\<RR> \<G>)" "fst r = \<SS> \<G>"
+  shows "wf_item \<G> \<omega> (Item r 0 0 0)"
+  using assms unfolding wf_item_def by simp
 
 lemma wf_Scan:
-  "wf_items cfg inp I \<Longrightarrow> wf_items cfg inp (Scan k inp I)"
-  unfolding Scan_def wf_defs bin_def inc_item_def is_complete_def item_rule_body_def next_symbol_def
-  by (auto split: if_splits)
+  assumes "x = Item r b i j" "wf_item \<G> \<omega> x" "\<omega>!j = a" "j < length \<omega>" "next_symbol x = Some a"
+  shows "wf_item \<G> \<omega> (Item r (b + 1) i (j+1))"
+  using assms unfolding wf_item_def by (auto simp: item_defs is_complete_def next_symbol_def split: if_splits)
 
 lemma wf_Predict:
-  "wf_items cfg inp I \<Longrightarrow> wf_items cfg inp (Predict k cfg I)"
-  unfolding Predict_def wf_defs bin_def init_item_def by auto
+  assumes "x = Item r b i j" "wf_item \<G> \<omega> x" "r' \<in> set (\<RR> \<G>)" "next_symbol x = Some (rule_head r')"
+  shows "wf_item \<G> \<omega> (Item r' 0 j j)"
+  using assms unfolding wf_item_def by simp
 
 lemma wf_Complete:
-  "wf_items cfg inp I \<Longrightarrow> wf_items cfg inp (Complete k I)"
-  unfolding Complete_def wf_defs bin_def inc_item_def is_complete_def item_rule_body_def next_symbol_def
-  by (auto split: if_splits; metis le_trans)
+  assumes "x = Item r\<^sub>x b\<^sub>x i j" "wf_item \<G> \<omega> x" "y = Item r\<^sub>y b\<^sub>y j k" "wf_item \<G> \<omega> y"
+  assumes "is_complete y" "next_symbol x = Some (item_rule_head y)"
+  shows "wf_item \<G> \<omega> (Item r\<^sub>x (b\<^sub>x + 1) i k)"
+  using assms unfolding wf_item_def is_complete_def next_symbol_def item_rule_body_def
+  by (auto split: if_splits)
 
-lemma wf_\<pi>_step:
-  "wf_items cfg inp I \<Longrightarrow> wf_items cfg inp (\<pi>_step k cfg inp I)"
-  unfolding \<pi>_step_def using wf_Scan wf_Predict wf_Complete wf_items_Un by metis
-
-lemma wf_funpower:
-  "wf_items cfg inp I \<Longrightarrow> wf_items cfg inp (funpower (\<pi>_step k cfg inp) n I)"
-  using wf_\<pi>_step unfolding wf_items_def
-  by (induction n) (auto, blast)
-
-lemma wf_\<pi>:
-  "wf_items cfg inp I \<Longrightarrow> wf_items cfg inp (\<pi> k cfg inp I)"
-  by (metis \<pi>_def elem_limit_simp wf_funpower wf_items_def)
-
-lemma wf_\<pi>0:
-  "wf_items cfg inp (\<pi> 0 cfg inp (Init cfg))"
-  using wf_items_def wf_Init wf_\<pi> by metis
-
-lemma wf_\<I>:
-  "wf_items cfg inp (\<I> n cfg inp)"
-  by (induction n) (auto simp: wf_\<pi>0 wf_\<pi>)
-
-lemma wf_\<II>:
-  "wf_items cfg inp (\<II> cfg inp)"
-  unfolding \<II>_def using wf_\<I> by blast
+lemma wf_Earley:
+  assumes "x \<in> Earley \<G> \<omega>"
+  shows "wf_item \<G> \<omega> x"
+  using assms wf_Init wf_Scan wf_Predict wf_Complete
+  by (induction rule: Earley.induct) fast+
 
 
 subsection \<open>Soundness\<close>
 
 definition sound_item :: "'a cfg \<Rightarrow> 'a sentence \<Rightarrow> 'a item \<Rightarrow> bool" where
-  "sound_item cfg inp x = derives cfg [item_rule_head x] (slice (item_origin x) (item_end x) inp @ item_\<beta> x)"
-
-definition sound_items :: "'a cfg \<Rightarrow> 'a sentence \<Rightarrow> 'a items \<Rightarrow> bool" where
-  "sound_items cfg inp I = (\<forall>x \<in> I. sound_item cfg inp x)"
-
-lemmas sound_defs = sound_items_def sound_item_def
+  "sound_item \<G> \<omega> x = derives \<G> [item_rule_head x] (slice (item_origin x) (item_end x) \<omega> @ item_\<beta> x)"
 
 lemma sound_Init:
-  "sound_items cfg inp (Init cfg)"
-  unfolding sound_items_def
-proof (standard)
-  fix x
-  assume *: "x \<in> Init cfg"
-  hence "item_dot x = 0"
-    by (smt (verit) Init_def init_item_def item.exhaust_sel item.inject mem_Collect_eq)
-  hence "(item_rule_head x, item_\<beta> x) \<in> set (\<RR> cfg)"
-    unfolding item_rule_head_def rule_head_def item_\<beta>_def item_rule_body_def rule_body_def
-    using * wf_Init wf_item_def by fastforce
-  hence "derives cfg [item_rule_head x] (item_\<beta> x)"
+  assumes "r \<in> set (\<RR> \<G>)" "fst r = \<SS> \<G>"
+  shows "sound_item \<G> \<omega> (Item r 0 0 0)"
+proof -
+  let ?x = "Item r 0 0 0"
+  have "(item_rule_head ?x, item_\<beta> ?x) \<in> set (\<RR> \<G>)"
+    using assms(1) by (simp add: item_defs)
+  hence "derives \<G> [item_rule_head ?x] (item_\<beta> ?x)"
     using derives_if_valid_rule by metis
-  moreover have "item_origin x = item_end x"
-    by (metis * Ex_list_of_length nle_le wf_Init wf_item_def)
-  ultimately show "sound_item cfg inp x"
+  thus "sound_item \<G> \<omega> ?x"
     unfolding sound_item_def by (simp add: slice_empty)
 qed
 
-lemma sound_item_inc_item:
-  assumes "wf_item cfg inp x" "sound_item cfg inp x"
-  assumes "next_symbol x = Some a"
-  assumes "k < length inp" "inp!k = a" "item_end x = k"
-  shows "sound_item cfg inp (inc_item x (k+1))"
-proof -
-  define x' where [simp]: "x' = inc_item x (k+1)"
-  obtain item_\<beta>' where *: "item_\<beta> x = a # item_\<beta>'"
-    using assms(3) apply (auto simp: item_\<beta>_def is_complete_def next_symbol_def split: if_splits)
-    by (metis Cons_nth_drop_Suc leI)
-  have "slice (item_origin x) (item_end x) inp @ item_\<beta> x = slice (item_origin x') (item_end x') inp @ item_\<beta>'"
-    using * assms(1,4-6) slice_append_nth wf_item_def by (auto simp: inc_item_def; blast)
-  moreover have "item_\<beta>' = item_\<beta> x'"
-    using * by (auto simp: inc_item_def item_\<beta>_def item_rule_body_def, metis List.list.sel(3) drop_Suc tl_drop)
-  moreover have "derives cfg [item_rule_head x] (slice (item_origin x) (item_end x) inp @ item_\<beta> x)"
-    using assms(1,2,6) sound_item_def by blast
-  ultimately show ?thesis
-    by (simp add: inc_item_def item_rule_head_def sound_item_def)
-qed
-
 lemma sound_Scan:
-  "wf_items cfg inp I \<Longrightarrow> sound_items cfg inp I \<Longrightarrow> sound_items cfg inp (Scan k inp I)"
-  unfolding Scan_def using sound_item_inc_item by (auto simp: wf_items_def sound_items_def bin_def; fast)
+  assumes "x = Item r b i j" "wf_item \<G> \<omega> x" "sound_item \<G> \<omega> x"
+  assumes "\<omega>!j = a" "j < length \<omega>" "next_symbol x = Some a"
+  shows "sound_item \<G> \<omega> (Item r (b+1) i (j+1))"
+proof -
+  define x' where [simp]: "x' = Item r (b+1) i (j+1)"
+  obtain item_\<beta>' where *: "item_\<beta> x = a # item_\<beta>'" "item_\<beta> x' = item_\<beta>'"
+    using assms(1,6) apply (auto simp: item_defs next_symbol_def is_complete_def split: if_splits)
+    by (metis Cons_nth_drop_Suc leI)
+  have "slice i j \<omega> @ item_\<beta> x = slice i (j+1) \<omega> @ item_\<beta>'"
+    using * assms(1,2,4,5) by (auto simp: slice_append_nth wf_item_def)
+  moreover have "derives \<G> [item_rule_head x] (slice i j \<omega> @ item_\<beta> x)"
+    using assms(1,3) sound_item_def by force
+  ultimately show ?thesis
+    using assms(1) * by (auto simp: item_defs sound_item_def)
+qed
 
 lemma sound_Predict:
-  "sound_items cfg inp I \<Longrightarrow> sound_items cfg inp (Predict k cfg I)"
-  unfolding Predict_def by (auto simp: sound_defs init_item_def derives_if_valid_rule slice_empty item_defs)
+  assumes "x = Item r b i j" "wf_item \<G> \<omega> x" "sound_item \<G> \<omega> x"
+  assumes "r' \<in> set (\<RR> \<G>)" "next_symbol x = Some (rule_head r')"
+  shows "sound_item \<G> \<omega> (Item r' 0 j j)"
+  using assms by (auto simp: sound_item_def derives_if_valid_rule slice_empty item_defs)
 
 lemma sound_Complete:
-  assumes "wf_items cfg inp I" "sound_items cfg inp I"
-  shows "sound_items cfg inp (Complete k I)"
-  unfolding sound_items_def
-proof standard
-  fix z
-  assume "z \<in> Complete k I"
-  show "sound_item cfg inp z"
-  proof cases
-    assume "z \<in> I"
-    thus ?thesis
-      using assms unfolding sound_items_def by blast
-  next
-    assume "\<not> z \<in> I"
-    then obtain x y where *:
-      "z = inc_item x k" "x \<in> bin I (item_origin y)" "y \<in> bin I k" 
-      "is_complete y" "next_symbol x = Some (item_rule_head y)"
-      using \<open>z \<in> Complete k I\<close> unfolding Complete_def by blast
-
-    have "derives cfg [item_rule_head y] (slice (item_origin y) (item_end y) inp)"
-      using *(3,4) sound_defs assms
-      by (metis (no_types, lifting) append_Nil2 bin_def drop_eq_Nil is_complete_def item_\<beta>_def mem_Collect_eq)
-    then obtain E where E: "Derivation cfg [item_rule_head y] E (slice (item_origin y) (item_end y) inp)"
-      using derives_implies_Derivation by blast
-
-    have "derives cfg [item_rule_head x] (slice (item_origin x) (item_origin y) inp @ item_\<beta> x)"
-      using *(2) sound_defs assms sound_items_def by (metis (mono_tags, lifting) bin_def mem_Collect_eq)
-    moreover have 0: "item_\<beta> x = (item_rule_head y) # tl (item_\<beta> x)"
-      using *(5) by (auto simp: next_symbol_def item_\<beta>_def is_complete_def split: if_splits,
-                     metis Cons_nth_drop_Suc drop_Suc drop_tl leI)
-    ultimately obtain D where D: 
-      "Derivation cfg [item_rule_head x] D (slice (item_origin x) (item_origin y) inp @
-       [item_rule_head y] @ (tl (item_\<beta> x)))"
-      using derives_implies_Derivation by (metis append_Cons append_Nil)
-
-    have "wf_item cfg inp x"
-      using *(2) assms(1) bin_def wf_items_def by (metis (mono_tags, lifting) mem_Collect_eq)
-    obtain G where 
-      "Derivation cfg [item_rule_head x] G (slice (item_origin x) (item_origin y) inp @
-       slice (item_origin y) (item_end y) inp @ tl (item_\<beta> x))"
-      using Derivation_append_rewrite D E by blast
-    moreover have "item_origin x \<le> item_origin y"
-      using *(2) \<open>wf_item cfg inp x\<close> wf_item_def by (auto simp: bin_def; force)
-    moreover have "item_origin y \<le> item_end y"
-      using *(3) wf_defs assms(1) by (auto simp: bin_def; blast)
-    ultimately have "derives cfg [item_rule_head x] (slice (item_origin x) (item_end y) inp @ tl (item_\<beta> x))"
-      by (metis Derivation_implies_derives append.assoc slice_concat)
-    moreover have "tl (item_\<beta> x) = item_\<beta> z"
-      using *(1,5) 0 by (auto simp: inc_item_def item_rule_body_def tl_drop drop_Suc item_\<beta>_def)
-    ultimately show ?thesis
-      using sound_item_def *(1,3) by (metis (mono_tags, lifting) bin_def inc_item_def item.sel(1,3,4) item_defs(1) mem_Collect_eq)
-  qed
+  assumes "x = Item r\<^sub>x b\<^sub>x i j" "wf_item \<G> \<omega> x" "sound_item \<G> \<omega> x"
+  assumes "y = Item r\<^sub>y b\<^sub>y j k" "wf_item \<G> \<omega> y" "sound_item \<G> \<omega> y"
+  assumes "is_complete y" "next_symbol x = Some (item_rule_head y)"
+  shows "sound_item \<G> \<omega> (Item r\<^sub>x (b\<^sub>x + 1) i k)"
+proof -
+  have "derives \<G> [item_rule_head y] (slice j k \<omega>)"
+    using assms(4,6,7) by (auto simp: sound_item_def is_complete_def item_defs)
+  then obtain E where E: "Derivation \<G> [item_rule_head y] E (slice j k \<omega>)"
+    using derives_implies_Derivation by blast
+  have "derives \<G> [item_rule_head x] (slice i j \<omega> @ item_\<beta> x)"
+    using assms(1,3,4) by (auto simp: sound_item_def)
+  moreover have 0: "item_\<beta> x = (item_rule_head y) # tl (item_\<beta> x)"
+    using assms(8) apply (auto simp: next_symbol_def is_complete_def item_defs split: if_splits)
+    by (metis drop_eq_Nil hd_drop_conv_nth leI list.collapse)
+  ultimately obtain D where D: 
+    "Derivation \<G> [item_rule_head x] D (slice i j \<omega> @ [item_rule_head y] @ (tl (item_\<beta> x)))"
+    using derives_implies_Derivation by (metis append_Cons append_Nil)
+  obtain F where F:
+    "Derivation \<G> [item_rule_head x] F (slice i j \<omega> @ slice j k \<omega> @ tl (item_\<beta> x))"
+    using Derivation_append_rewrite D E by blast
+  moreover have "i \<le> j"
+    using assms(1,2) wf_item_def by force
+  moreover have "j \<le> k"
+    using assms(4,5) wf_item_def by force
+  ultimately have "derives \<G> [item_rule_head x] (slice i k \<omega> @ tl (item_\<beta> x))"
+    by (metis Derivation_implies_derives append.assoc slice_concat)
+  thus "sound_item \<G> \<omega> (Item r\<^sub>x (b\<^sub>x + 1) i k)"
+    using assms(1,4) by (auto simp: sound_item_def item_defs drop_Suc tl_drop)
 qed
 
-lemma sound_\<pi>_step:
-  "wf_items cfg inp I \<Longrightarrow> sound_items cfg inp I \<Longrightarrow> sound_items cfg inp (\<pi>_step k cfg inp I)"
-  unfolding \<pi>_step_def using sound_Scan sound_Predict sound_Complete by (metis UnE sound_items_def)
-
-lemma sound_funpower:
-  "wf_items cfg inp I \<Longrightarrow> sound_items cfg inp I \<Longrightarrow> sound_items cfg inp (funpower (\<pi>_step k cfg inp) n I)"
-  by (induction n) (auto simp: sound_\<pi>_step wf_\<pi>_step wf_funpower)
-
-lemma sound_\<pi>:
-  assumes "wf_items cfg inp I" "sound_items cfg inp I"
-  shows "sound_items cfg inp (\<pi> k cfg inp I)"
-  by (metis \<pi>_def assms elem_limit_simp sound_items_def sound_funpower)
-
-lemma sound_\<pi>0:
-  "sound_items cfg inp (\<pi> 0 cfg inp (Init cfg))"
-  using sound_Init sound_\<pi> wf_Init wf_items_def by metis
-
-lemma sound_\<I>:
-  "sound_items cfg inp (\<I> k cfg inp)"
-  apply (induction k)
-  apply (auto simp: sound_\<pi>0)
-  using sound_\<pi> wf_\<I> by force
-
-lemma sound_\<II>:
-  "sound_items cfg inp (\<II> cfg inp)"
-  unfolding \<II>_def using sound_\<I> by blast
+lemma sound_Earley:
+  assumes "x \<in> Earley \<G> \<omega>" "wf_item \<G> \<omega> x"
+  shows "sound_item \<G> \<omega> x"
+  using assms
+proof (induction rule: Earley.induct)
+  case (Init r)
+  thus ?case
+    using sound_Init by blast
+next
+  case (Scan x r b i j a)
+  thus ?case
+    using wf_Earley sound_Scan by fast
+next
+  case (Predict x r b i j r')
+  thus ?case
+    using wf_Earley sound_Predict  by blast
+next
+  case (Complete x r\<^sub>x b\<^sub>x i j y r\<^sub>y b\<^sub>y k)
+  thus ?case
+    using wf_Earley sound_Complete by metis
+qed
 
 theorem soundness:
-  "earley_recognized (\<II> cfg inp) cfg inp \<Longrightarrow> derives cfg [\<SS> cfg] inp"
-  using earley_recognized_def sound_\<II> sound_defs
-  by (metis drop_eq_Nil is_complete_def is_finished_def item_\<beta>_def self_append_conv slice_id)
-
-
-subsection \<open>Monotonicity and Absorption\<close>
-
-lemma \<pi>_step_empty:
-  "\<pi>_step k cfg inp {} = {}"
-  unfolding \<pi>_step_def Scan_def Complete_def Predict_def bin_def by blast
-
-lemma \<pi>_step_setmonotone:
-  "setmonotone (\<pi>_step k cfg inp)"
-  by (simp add: Un_assoc \<pi>_step_def setmonotone_def)
-
-lemma \<pi>_step_continuous:
-  "continuous (\<pi>_step k cfg inp)"
-  unfolding continuous_def
-proof (standard, standard, standard)
-  fix C :: "nat \<Rightarrow> 'a item set"
-  assume "chain C"
-  thus "chain (\<pi>_step k cfg inp \<circ> C)"
-    unfolding chain_def \<pi>_step_def by (auto simp: Scan_def Predict_def Complete_def bin_def subset_eq)
-next
-  fix C :: "nat \<Rightarrow> 'a item set"
-  assume *: "chain C"
-  show "\<pi>_step k cfg inp (natUnion C) = natUnion (\<pi>_step k cfg inp \<circ> C)"
-    unfolding natUnion_def
-  proof standard
-    show "\<pi>_step k cfg inp (\<Union> {C n |n. True}) \<subseteq> \<Union> {(\<pi>_step k cfg inp \<circ> C) n |n. True}"
-    proof standard
-      fix x
-      assume #: "x \<in> \<pi>_step k cfg inp (\<Union> {C n |n. True})"
-      show "x \<in> \<Union> {(\<pi>_step k cfg inp \<circ> C) n |n. True}"
-      proof (cases "x \<in> Complete k (\<Union> {C n |n. True})")
-        case True
-        then show ?thesis
-          using * unfolding chain_def
-          apply (auto simp: \<pi>_step_def Complete_def bin_def)
-        proof -
-          fix y :: "'a item" and z :: "'a item" and n :: nat and m :: nat
-          assume a1: "is_complete z"
-          assume a2: "item_end y = item_origin z"
-          assume a3: "y \<in> C n"
-          assume a4: "z \<in> C m"
-          assume a5: "next_symbol y = Some (item_rule_head z)"
-          assume "\<forall>i. C i \<subseteq> C (Suc i)"
-          hence f6: "\<And>n m. \<not> n \<le> m \<or> C n \<subseteq> C m"
-            by (meson lift_Suc_mono_le)
-          hence f7: "\<And>n. \<not> m \<le> n \<or> z \<in> C n"
-            using a4 by blast
-          have "\<exists>n \<ge> m. y \<in> C n"
-            using f6 a3 by (meson le_sup_iff subset_eq sup_ge1)
-          thus "\<exists>I.
-                  (\<exists>n. I = C n \<union> 
-                           Scan (item_end z) inp (C n) \<union> 
-                           {inc_item i (item_end z) |i. 
-                              i \<in> C n \<and> 
-                              (\<exists>j. 
-                                item_end i = item_origin j \<and>
-                                j \<in> C n \<and> 
-                                item_end j = item_end z \<and> 
-                                is_complete j \<and>
-                                next_symbol i = Some (item_rule_head j))} \<union>
-                           Predict (item_end z) cfg (C n))
-                  \<and> inc_item y (item_end z) \<in> I"
-            using f7 a5 a2 a1 by blast
-        qed
-      next
-        case False
-        thus ?thesis
-          using # Un_iff by (auto simp: \<pi>_step_def Scan_def Predict_def bin_def; blast)
-      qed
-    qed
-  next
-    show "\<Union> {(\<pi>_step k cfg inp \<circ> C) n |n. True} \<subseteq> \<pi>_step k cfg inp (\<Union> {C n |n. True})"
-      unfolding \<pi>_step_def
-      using * by (auto simp: Scan_def Predict_def Complete_def chain_def bin_def, metis+)
-  qed
-qed
-
-lemma \<pi>_step_regular:
-  "regular (\<pi>_step k cfg inp)"
-  by (simp add: \<pi>_step_continuous \<pi>_step_setmonotone regular_def)
-
-lemma \<pi>_idem:
-  "\<pi> k cfg inp (\<pi> k cfg inp I) = \<pi> k cfg inp I"
-  by (simp add: \<pi>_def \<pi>_step_regular limit_is_idempotent)
-
-lemma Scan_bin_absorb:
-  "Scan k inp (bin I k) = Scan k inp I"
-  unfolding Scan_def bin_def by simp
-
-lemma Predict_bin_absorb:
-  "Predict k cfg (bin I k) = Predict k cfg I"
-  unfolding Predict_def bin_def by simp
-
-lemma Complete_bin_absorb:
-  "Complete k (bin I k) \<subseteq> Complete k I"
-  unfolding Complete_def bin_def by blast
-
-lemma Scan_Un:
-  "Scan k inp (I \<union> J) = Scan k inp I \<union> Scan k inp J"
-  unfolding Scan_def bin_def by blast
-
-lemma Predict_Un:
-  "Predict k cfg (I \<union> J) = Predict k cfg I \<union> Predict k cfg J"
-  unfolding Predict_def bin_def by blast
-
-lemma Scan_sub_mono:
-  "I \<subseteq> J \<Longrightarrow> Scan k inp I \<subseteq> Scan k inp J"
-  unfolding Scan_def bin_def by blast
-
-lemma Predict_sub_mono:
-  "I \<subseteq> J \<Longrightarrow> Predict k cfg I \<subseteq> Predict k cfg J"
-  unfolding Predict_def bin_def by blast
-
-lemma Complete_sub_mono:
-  "I \<subseteq> J \<Longrightarrow> Complete k I \<subseteq> Complete k J"
-  unfolding Complete_def bin_def by blast
-
-lemma \<pi>_step_sub_mono:
-  "I \<subseteq> J \<Longrightarrow> \<pi>_step k cfg inp I \<subseteq> \<pi>_step k cfg inp J"
-  unfolding \<pi>_step_def using Scan_sub_mono Predict_sub_mono Complete_sub_mono by (metis sup.mono)
-
-lemma funpower_sub_mono:
-  "I \<subseteq> J \<Longrightarrow> funpower (\<pi>_step k cfg inp) n I \<subseteq> funpower (\<pi>_step k cfg inp) n J"
-  by (induction n) (auto simp: \<pi>_step_sub_mono)
-
-lemma \<pi>_sub_mono:
-  "I \<subseteq> J \<Longrightarrow> \<pi> k cfg inp I \<subseteq> \<pi> k cfg inp J"
-proof standard
-  fix x
-  assume "I \<subseteq> J" "x \<in> \<pi> k cfg inp I"
-  then obtain n where "x \<in> funpower (\<pi>_step k cfg inp) n I"
-    unfolding \<pi>_def limit_def natUnion_def by blast
-  hence "x \<in> funpower (\<pi>_step k cfg inp) n J"
-    using \<open>I \<subseteq> J\<close> funpower_sub_mono by blast
-  thus "x \<in> \<pi> k cfg inp J"
-    unfolding \<pi>_def limit_def natUnion_def by blast
-qed
-
-lemma Scan_\<pi>_step_mono:
-  "Scan k inp I \<subseteq> \<pi>_step k cfg inp I"
-  using \<pi>_step_def by blast
-
-lemma Predict_\<pi>_step_mono:
-  "Predict k cfg I \<subseteq> \<pi>_step k cfg inp I"
-  using \<pi>_step_def by blast
-
-lemma Complete_\<pi>_step_mono:
-  "Complete k I \<subseteq> \<pi>_step k cfg inp I"
-  using \<pi>_step_def by blast
-
-lemma \<pi>_step_\<pi>_mono:
-  "\<pi>_step k cfg inp I \<subseteq> \<pi> k cfg inp I"
+  assumes "earley_recognized (Earley \<G> \<omega>) \<G> \<omega>"
+  shows "derives \<G> [\<SS> \<G>] \<omega>"
 proof -
-  have "\<pi>_step k cfg inp I \<subseteq> funpower (\<pi>_step k cfg inp) 1 I"
-    by simp
+  obtain x where x: "x \<in> Earley \<G> \<omega>" "is_finished \<G> \<omega> x"
+    using assms earley_recognized_def by blast
+  hence "sound_item \<G> \<omega> x"
+    using wf_Earley sound_Earley by blast
   thus ?thesis
-    by (metis \<pi>_def limit_elem subset_eq)
-qed
-
-lemma Scan_\<pi>_mono:
-  "Scan k inp  I \<subseteq> \<pi> k cfg inp I"
-  using Scan_\<pi>_step_mono \<pi>_step_\<pi>_mono by force
-
-lemma Predict_\<pi>_mono:
-  "Predict k cfg I \<subseteq> \<pi> k cfg inp I"
-  using Predict_\<pi>_step_mono \<pi>_step_\<pi>_mono by force
-
-lemma Complete_\<pi>_mono:
-  "Complete k I \<subseteq> \<pi> k cfg inp I"
-  using Complete_\<pi>_step_mono \<pi>_step_\<pi>_mono by force
-
-lemma \<pi>_mono:
-  "I \<subseteq> \<pi> k cfg inp I"
-  using \<pi>_step_\<pi>_mono \<pi>_step_def by blast
-
-lemma Scan_bin_empty:
-  "i \<noteq> k \<Longrightarrow> i \<noteq> k+1 \<Longrightarrow> bin (Scan k inp I) i = {}"
-  unfolding Scan_def bin_def inc_item_def by fastforce
-
-lemma Predict_bin_empty:
-  "i \<noteq> k \<Longrightarrow> bin (Predict k cfg I) i = {}"
-  unfolding Predict_def bin_def init_item_def by auto
-
-lemma Complete_bin_empty:
-  "i \<noteq> k \<Longrightarrow> bin (Complete k I) i = {}"
-  unfolding Complete_def bin_def inc_item_def by auto
-
-lemma \<pi>_step_bin_absorb:
-  "i \<noteq> k \<Longrightarrow> i \<noteq> k + 1 \<Longrightarrow> bin (\<pi>_step k cfg inp I) i = bin I i"
-  unfolding \<pi>_step_def using Scan_bin_empty Predict_bin_empty Complete_bin_empty
-  unfolding bin_def using Un_iff empty_iff mem_Collect_eq by fastforce
-
-lemma funpower_bin_absorb:
-  "i \<noteq> k \<Longrightarrow> i \<noteq> k+1 \<Longrightarrow> bin (funpower (\<pi>_step k cfg inp) n I) i = bin I i"
-  by (induction n) (auto simp: \<pi>_step_bin_absorb)
-
-lemma \<pi>_bin_absorb:
-  assumes "i \<noteq> k" "i \<noteq> k+1" 
-  shows "bin (\<pi> k cfg inp I) i = bin I i"
-proof (standard; standard)
-  fix x 
-  assume "x \<in> bin (\<pi> k cfg inp I) i"
-  then obtain n where "x \<in> bin (funpower (\<pi>_step k cfg inp) n I) i"
-    unfolding \<pi>_def limit_def natUnion_def by (auto simp: bin_def)
-  then show "x \<in> bin I i"
-    using funpower_bin_absorb assms by blast
-next
-  fix x
-  assume "x \<in> bin I i"
-  show "x \<in> bin (\<pi> k cfg inp I) i"
-    using \<pi>_mono \<open>x \<in> bin I i\<close> by (metis (no_types, lifting) bin_def mem_Collect_eq subsetD)
+    unfolding sound_item_def using x by (auto simp: is_finished_def is_complete_def item_defs)
 qed
 
 
 subsection \<open>Completeness\<close>
 
-lemma Scan_\<I>:
-  assumes "i+1 \<le> k" "k \<le> length inp" "x \<in> bin (\<I> k cfg inp) i" "next_symbol x = Some a" "inp!i = a"
-  shows "inc_item x (i+1) \<in> \<I> k cfg inp"
-  using assms
-proof (induction k arbitrary: i x a)
-  case 0
-  have False
-    using "0.prems"(1) by simp
-  thus ?case
-    by blast
-next
-  case (Suc k)
-  have "bin (\<I> (k+1) cfg inp) i = bin (\<pi> (k+1) cfg inp (\<I> k cfg inp)) i"
-    by simp
-  also have "... = bin (\<I> k cfg inp) i"
-    using \<pi>_bin_absorb Suc.prems(1) by (metis Suc_eq_plus1 add_le_same_cancel1 not_one_le_zero trans_le_add1)
-  finally have "bin (\<I> (k+1) cfg inp) i = bin (\<I> k cfg inp) i" .
-  hence *: "x \<in> bin (\<I> k cfg inp) i"
-    using Suc.prems(3) by force
-  show ?case
-  proof cases
-    assume "i+1 \<le> k"
-    hence "inc_item x (i+1) \<in> \<I> k cfg inp"
-      using Suc.IH Suc.prems(2,4,5) * by simp
-    thus ?thesis
-      using \<pi>_mono by force
-  next
-    assume "\<not> i+1 \<le> k"
-    hence "i = k"
-      using Suc.prems(1) by auto
-    hence "inc_item x (i+1) \<in> Scan k inp (\<I> k cfg inp)"
-      using Suc.prems(2,4,5) * Scan_def by force
-    hence "inc_item x (i+1) \<in> \<pi> k cfg inp (\<I> k cfg inp)"
-      using Scan_\<pi>_mono by blast
-    hence "inc_item x (i+1) \<in> \<I> k cfg inp"
-      using \<pi>_idem by (metis \<I>.elims)
-    thus ?thesis
-      using \<pi>_mono by force
-  qed
-qed
-
-lemma Predict_\<I>:
-  assumes "i \<le> k" "x \<in> bin (\<I> k cfg inp) i" "next_symbol x = Some N" "(N,\<alpha>) \<in> set (\<RR> cfg)"
-  shows "init_item (N,\<alpha>) i \<in> \<I> k cfg inp"
-  using assms
-proof (induction k arbitrary: i x N \<alpha>)
-  case 0
-  hence "init_item (N,\<alpha>) i \<in> Predict 0 cfg (\<I> 0 cfg inp)"
-    unfolding rule_head_def Predict_def by auto
-  thus ?case
-    using Predict_\<pi>_mono \<pi>_idem by fastforce
-next
-  case (Suc k)
-  show ?case
-  proof cases
-    assume "i \<le> k"
-    hence "init_item (N,\<alpha>) i \<in> \<I> k cfg inp"
-      using Suc.IH \<pi>_bin_absorb Suc.prems(2-4) by (metis \<I>.simps(2) add.commute le_imp_less_Suc nless_le plus_1_eq_Suc)
-    thus ?thesis
-      using \<pi>_mono by fastforce
-  next
-    assume "\<not> i \<le> k"
-    hence "init_item (N,\<alpha>) i \<in> Predict i cfg (\<I> (Suc k) cfg inp)"
-      unfolding Predict_def rule_head_def using Suc.prems(2-4) by auto
-    thus ?thesis
-      using Predict_\<pi>_mono \<pi>_idem Suc.prems(1) \<open>\<not> i \<le> k\<close> by (metis le_SucE \<I>.simps(2) subsetD)
-  qed
-qed
-
-lemma Complete_\<I>:
-  assumes "i \<le> j" "j \<le> k" "x \<in> bin (\<I> k cfg inp) i" "next_symbol x = Some N" "(N,\<alpha>) \<in> set (\<RR> cfg)"
-  assumes "i = item_origin y" "y \<in> bin (\<I> k cfg inp) j" "item_rule y = (N,\<alpha>)" "is_complete y"
-  shows "inc_item x j \<in> \<I> k cfg inp"
-  using assms
-proof (induction k arbitrary: i j x N \<alpha> y)
-  case 0
-  hence "inc_item x 0 \<in> Complete 0 (\<I> 0 cfg inp)"
-    unfolding Complete_def rule_head_def next_symbol_def item_rule_head_def by (auto split: if_splits; force)
-  thus ?case
-    using Complete_\<pi>_mono \<pi>_idem "0.prems"(2) by (metis le_0_eq \<I>.simps(1) subset_iff)
-next
-  case (Suc k)
-  show ?case
-  proof cases
-    assume "j \<le> k"
-    hence "inc_item x j \<in> \<I> k cfg inp"
-      using Suc  \<pi>_bin_absorb Orderings.order_class.dual_order.eq_iff by (metis Suc_eq_plus1 \<I>.simps(2) not_less_eq_eq)
-    thus ?thesis
-      using \<pi>_mono by fastforce
-  next
-    assume "\<not> j \<le> k"
-    hence "j = Suc k"
-      using le_SucE Suc.prems(2) by blast
-    hence "inc_item x (Suc k) \<in> Complete (Suc k) (\<I> (Suc k) cfg inp)"
-      using Suc.prems(3-4,6-9) unfolding Complete_def rule_head_def item_rule_head_def by fastforce
-    then show ?thesis
-      using Complete_\<pi>_mono \<pi>_idem \<open>j = Suc k\<close> by fastforce
-  qed
-qed
-
-definition partially_completed :: "nat \<Rightarrow> 'a cfg \<Rightarrow> 'a sentence \<Rightarrow> 'a items \<Rightarrow> ('a derivation \<Rightarrow> bool) \<Rightarrow> bool" where
-  "partially_completed k cfg inp I P = (
-    \<forall>i j x a D.
-      i \<le> j \<and> j \<le> k \<and> k \<le> length inp \<and>
-      x \<in> bin I i \<and> next_symbol x = Some a \<and>
-      Derivation cfg [a] D (slice i j inp) \<and> P D \<longrightarrow>
-      inc_item x j \<in> I
+definition partially_completed :: "nat \<Rightarrow> 'a cfg \<Rightarrow> 'a sentence \<Rightarrow> 'a item set \<Rightarrow> ('a derivation \<Rightarrow> bool) \<Rightarrow> bool" where
+  "partially_completed k \<G> \<omega> E P = (
+    \<forall>r b i' i j x a D.
+      i \<le> j \<and> j \<le> k \<and> k \<le> length \<omega> \<and>
+      x = Item r b i' i \<and> x \<in> E \<and> next_symbol x = Some a \<and>
+      Derivation \<G> [a] D (slice i j \<omega>) \<and> P D \<longrightarrow>
+      Item r (b+1) i' j \<in> E
   )"
 
-lemma fully_completed:
-  assumes "j \<le> k" "k \<le> length inp"
-  assumes "x = Item (N,\<alpha>) d i j" "x \<in> I" "wf_items cfg inp I"
-  assumes "Derivation cfg (item_\<beta> x) D (slice j k inp)"
-  assumes "partially_completed k cfg inp I (\<lambda>D'. length D' \<le> length D)"
+lemma partially_completed_upto:
+  assumes "j \<le> k" "k \<le> length \<omega>"
+  assumes "x = Item (N,\<alpha>) d i j" "x \<in> I" "\<forall>x \<in> I. wf_item \<G> \<omega> x"
+  assumes "Derivation \<G> (item_\<beta> x) D (slice j k \<omega>)"
+  assumes "partially_completed k \<G> \<omega> I (\<lambda>D'. length D' \<le> length D)"
   shows "Item (N,\<alpha>) (length \<alpha>) i k \<in> I"
   using assms
 proof (induction "item_\<beta> x" arbitrary: d i j k N \<alpha> x D)
@@ -922,11 +442,10 @@ proof (induction "item_\<beta> x" arbitrary: d i j k N \<alpha> x D)
   have "item_\<alpha> x = \<alpha>"
     using Nil(1,4) unfolding item_\<alpha>_def item_\<beta>_def item_rule_body_def rule_body_def by simp
   hence "x = Item (N,\<alpha>) (length \<alpha>) i j"
-    using Nil.hyps Nil.prems(3,4,5)
-    unfolding wf_items_def wf_item_def rule_body_def item_rule_body_def item_defs(4) by auto
-  have "Derivation cfg [] D (slice j k inp)"
-    using Nil.hyps Nil.prems(6) by simp
-  hence "slice j k inp = []"
+    using Nil.hyps Nil.prems(3-5) unfolding wf_item_def item_defs by auto
+  have "Derivation \<G> [] D (slice j k \<omega>)"
+    using Nil.hyps Nil.prems(6) by auto
+  hence "slice j k \<omega> = []"
     using Derivation_from_empty by blast
   hence "j = k"
     unfolding slice_drop_take using Nil.prems(1,2) by simp
@@ -935,160 +454,183 @@ proof (induction "item_\<beta> x" arbitrary: d i j k N \<alpha> x D)
 next
   case (Cons b bs)
   obtain j' E F where *: 
-    "Derivation cfg [b] E (slice j j' inp)"
-    "Derivation cfg bs F (slice j' k inp)"
+    "Derivation \<G> [b] E (slice j j' \<omega>)"
+    "Derivation \<G> bs F (slice j' k \<omega>)"
     "j \<le> j'" "j' \<le> k" "length E \<le> length D" "length F \<le> length D"
-    using Derivation_concat_split[of cfg "[b]" bs D "slice j k inp"] slice_concat_Ex
+    using Derivation_concat_split[of \<G> "[b]" bs D "slice j k \<omega>"] slice_concat_Ex
     using Cons.hyps(2) Cons.prems(1,6)
     by (smt (verit, ccfv_threshold) Cons_eq_appendI append_self_conv2)
-  have "x \<in> bin I j"
-    using Cons.prems(3,4) by (auto simp: bin_def)
-  moreover have "next_symbol x = Some b"
+  have "next_symbol x = Some b"
     using Cons.hyps(2) unfolding item_defs(4) next_symbol_def is_complete_def by (auto, metis nth_via_drop)
-  ultimately have "inc_item x j' \<in> I"
-    using *(1,3-5) Cons.prems(2-4,7) partially_completed_def by metis
-
-  moreover have "partially_completed k cfg inp I (\<lambda>D'. length D' \<le> length F)"
+  hence "Item (N, \<alpha>) (d+1) i j' \<in> I"
+    using Cons.prems(7) unfolding partially_completed_def
+    using Cons.prems(2,3,4) *(1,3-5) by blast
+  moreover have "partially_completed k \<G> \<omega> I (\<lambda>D'. length D' \<le> length F)"
     using Cons.prems(7) *(6) unfolding partially_completed_def by fastforce
   moreover have "bs = item_\<beta> (Item (N,\<alpha>) (d+1) i j')"
     using Cons.hyps(2) Cons.prems(3) unfolding item_defs(4) item_rule_body_def 
     by (auto, metis List.list.sel(3) drop_Suc drop_tl)
   ultimately show ?case
-    using Cons.hyps(1) *(2,4) Cons.prems(2,3,5) wf_items_def by (auto simp: inc_item_def)
+    using Cons.hyps(1) *(2,4) Cons.prems(2,3,5) wf_item_def by blast
 qed
 
-lemma partially_completed_\<I>:
-  assumes "wf_cfg cfg"
-  shows "partially_completed k cfg inp (\<I> k cfg inp) (\<lambda>_. True)"
+lemma partially_completed_Earley_k:
+  assumes "wf_cfg \<G>"
+  shows "partially_completed k \<G> \<omega> (Earley \<G> \<omega>) (\<lambda>_. True)"
   unfolding partially_completed_def
-proof (standard, standard, standard, standard, standard, standard)
-  fix x i a D j
+proof (standard, standard, standard, standard, standard, standard, standard, standard, standard)
+  fix r b i' i j x a D
   assume
-    "i \<le> j \<and> j \<le> k \<and> k \<le> length inp \<and>
-     x \<in> bin (\<I> k cfg inp) i \<and> next_symbol x = Some a \<and>
-     Derivation cfg [a] D (slice i j inp) \<and> (\<lambda>_. True) D"
-  thus "inc_item x j \<in> \<I> k cfg inp"
-  proof (induction "length D" arbitrary: x i a j D rule: nat_less_induct)
+    "i \<le> j \<and> j \<le> k \<and> k \<le> length \<omega> \<and>
+     x = Item r b i' i \<and> x \<in> Earley \<G> \<omega> \<and>
+     next_symbol x = Some a \<and>
+     Derivation \<G> [a] D (slice i j \<omega>) \<and> True"
+  thus "Item r (b + 1) i' j \<in> Earley \<G> \<omega>"
+  proof (induction "length D" arbitrary: r b i' i j x a D rule: nat_less_induct)
     case 1
     show ?case
     proof cases
       assume "D = []"
-      hence "[a] = slice i j inp"
+      hence "[a] = slice i j \<omega>"
         using "1.prems" by force
-      moreover have "j \<le> length inp"
+      moreover have "j \<le> length \<omega>"
         using le_trans "1.prems" by blast
       ultimately have "j = i+1"
         using slice_singleton by metis
-      hence "i < length inp"
-        using \<open>j \<le> length inp\<close> discrete by blast
-      hence "inp!i = a"
-        using slice_nth \<open>[a] = slice i j inp\<close> \<open>j = i + 1\<close> by fastforce
-      hence "inc_item x (i+1) \<in> \<I> k cfg inp"
-        using Scan_\<I> \<open>j = i + 1\<close> "1.prems" by fast
+      hence "i < length \<omega>"
+        using \<open>j \<le> length \<omega>\<close> discrete by blast
+      hence "\<omega>!i = a"
+        using slice_nth \<open>[a] = slice i j \<omega>\<close> \<open>j = i + 1\<close> by fastforce
+      hence "Item r (b + 1) i' j \<in> Earley \<G> \<omega>"
+        using Earley.Scan "1.prems" \<open>i < length \<omega>\<close> \<open>j = i + 1\<close> by metis
       thus ?thesis
         by (simp add: \<open>j = i + 1\<close>)
     next
       assume "\<not> D = []"
       then obtain d D' where "D = d # D'"
         by (meson List.list.exhaust)
-      then obtain b where *: "Derives1 cfg [a] (fst d) (snd d) b" "Derivation cfg b D' (slice i j inp)"
+      then obtain \<alpha> where *: "Derives1 \<G> [a] (fst d) (snd d) \<alpha>" "Derivation \<G> \<alpha> D' (slice i j \<omega>)"
         using "1.prems" by auto
+      hence rule: "(a, \<alpha>) \<in> set (\<RR> \<G>)" "fst d = 0" "snd d = (a ,\<alpha>)"
+          using *(1) unfolding Derives1_def by (simp add: Cons_eq_append_conv)+
       show ?thesis
       proof cases
-        assume "is_terminal cfg a"
-        then obtain N \<alpha> where "[a] = [N]" "(N,\<alpha>) \<in> set (\<RR> cfg)"
-          using *(1) unfolding Derives1_def by (metis Cons_eq_append_conv neq_Nil_conv)
-         hence "is_nonterminal cfg a"
-           by (simp add: assms)
-         thus ?thesis
-          using \<open>is_terminal cfg a\<close> is_terminal_nonterminal by (metis assms)
+        assume "is_terminal \<G> a"
+        have "is_nonterminal \<G> a"
+          using rule by (simp add: assms)
+        thus ?thesis
+          using \<open>is_terminal \<G> a\<close> is_terminal_nonterminal by (metis assms)
       next
-        assume "\<not> is_terminal cfg a"
-        then obtain N \<alpha> where #: "[a] = [N]" "b = \<alpha>" "(N,\<alpha>) \<in> set (\<RR> cfg)" "fst d = 0" "snd d = (N,\<alpha>)"
-          using *(1) unfolding Derives1_def by (simp add: Cons_eq_append_conv)
-        define y where y_def: "y = Item (N,\<alpha>) 0 i i"
-        have "y \<in> \<I> k cfg inp"
-          using Predict_\<I> #(1,3) "1.prems" y_def init_item_def
-          by (metis (no_types, lifting) le_trans list.inject)
+        assume "\<not> is_terminal \<G> a"
+        define y where y_def: "y = Item (a ,\<alpha>) 0 i i"
+        have "y \<in> Earley \<G> \<omega>"
+          using y_def "1.prems" rule by (auto simp: item_defs Earley.Predict)
         have "i \<le> j"
           using "1.prems" by blast
-        have "j \<le> length inp"
+        have "j \<le> length \<omega>"
           using "1.prems" by simp
         have "length D' < length D"
           using \<open>D = d # D'\<close> by fastforce
-        hence "partially_completed k cfg inp (\<I> k cfg inp) (\<lambda>E. length E \<le> length D')"
-          unfolding partially_completed_def using "1.hyps" "1.prems" le_less_trans by blast
-        hence 0: "partially_completed j cfg inp (\<I> k cfg inp) (\<lambda>E. length E \<le> length D')"
+
+        have "\<forall>m<length D.
+     \<forall>x. m = length x \<longrightarrow>
+         (\<forall>xa xb xc xd xe xf xg.
+             xd \<le> xe \<and> xe \<le> k \<and> k \<le> length \<omega> \<and> xf = Item xa xb xc xd \<and> xf \<in> Earley \<G> \<omega> \<and> next_symbol xf = Some xg
+              \<and> Derivation \<G> [xg] x (slice xd xe \<omega>) \<and> True \<longrightarrow>
+             Item xa (xb + 1) xc xe \<in> Earley \<G> \<omega>)"
+          using "1.hyps" by blast
+        hence "\<forall>m x.
+      m < length D \<and> m = length x \<longrightarrow>
+         (\<forall>xa xb xc xd xe xf xg.
+             xd \<le> xe \<and> xe \<le> k \<and> k \<le> length \<omega> \<and> xf = Item xa xb xc xd \<and> xf \<in> Earley \<G> \<omega> \<and> next_symbol xf = Some xg
+              \<and> Derivation \<G> [xg] x (slice xd xe \<omega>) \<and> True \<longrightarrow>
+             Item xa (xb + 1) xc xe \<in> Earley \<G> \<omega>)"
+          by blast
+        hence "\<forall>m x.
+      m \<le> length D' \<and> m = length x \<longrightarrow>
+         (\<forall>xa xb xc xd xe xf xg.
+             xd \<le> xe \<and> xe \<le> k \<and> k \<le> length \<omega> \<and> xf = Item xa xb xc xd \<and> xf \<in> Earley \<G> \<omega> \<and> next_symbol xf = Some xg
+              \<and> Derivation \<G> [xg] x (slice xd xe \<omega>) \<and> True \<longrightarrow>
+             Item xa (xb + 1) xc xe \<in> Earley \<G> \<omega>)"
+          by (smt (verit, best) \<open>length D' < length D\<close> order_le_less_trans)
+        hence "\<forall>x.
+         (\<forall>xa xb xc xd xe xf xg.
+             xd \<le> xe \<and> xe \<le> k \<and> k \<le> length \<omega> \<and> xf = Item xa xb xc xd \<and> xf \<in> Earley \<G> \<omega> \<and> next_symbol xf = Some xg
+              \<and> Derivation \<G> [xg] x (slice xd xe \<omega>) \<and> length x \<le> length D' \<longrightarrow>
+             Item xa (xb + 1) xc xe \<in> Earley \<G> \<omega>)"
+          by fast
+        hence "partially_completed k \<G> \<omega> (Earley \<G> \<omega>) (\<lambda>E. length E \<le> length D')"
+          unfolding partially_completed_def by blast
+        hence 0: "partially_completed j \<G> \<omega> (Earley \<G> \<omega>) (\<lambda>E. length E \<le> length D')"
           unfolding partially_completed_def using "1.prems" by force
-        have 1: "Derivation cfg (item_\<beta> y) D' (slice i j inp)"
-          using #(2) *(2) item_\<beta>_def item_rule_body_def rule_body_def y_def
-          by (metis item.sel(1) item.sel(2) drop0 snd_conv)
-        have 0: "Item (N,\<alpha>) (length \<alpha>) i j \<in> bin (\<I> k cfg inp) j"
-          using fully_completed[OF \<open>i \<le> j\<close> \<open>j \<le> length inp\<close> y_def \<open>y \<in> \<I> k cfg inp\<close> wf_\<I> 1 0] bin_def
-          by force
-        have 1: "x \<in> bin (\<I> k cfg inp) i"
-          by (simp add: "1.prems")
+
+        have 1: "Derivation \<G> (item_\<beta> y) D' (slice i j \<omega>)"
+          using *(2) by (auto simp: item_defs y_def)
+        have 0: "Item (a,\<alpha>) (length \<alpha>) i j \<in> Earley \<G> \<omega>"
+          using partially_completed_upto by (metis "0" "1" "1.prems" \<open>j \<le> length \<omega>\<close> \<open>y \<in> Earley \<G> \<omega>\<close> wf_Earley y_def)
+
+        have 2: "x = Item r b i' i" "x \<in> Earley \<G> \<omega>"
+          using "1.prems" by blast+
+
         have "j \<le> k"
           using "1.prems" by blast
-        have "next_symbol x = Some N"
-          using #(1) "1.prems" by fastforce
+        have "next_symbol x = Some a"
+          using "1.prems" by linarith
         thus ?thesis
-          using "1.prems" Complete_\<I>[OF \<open>i \<le> j\<close> \<open>j \<le> k\<close> 1 \<open>next_symbol x = Some N\<close> #(3) _ 0] by (auto simp: is_complete_def item_rule_body_def rule_body_def)
+          using Earley.Complete[OF 2 _ 0] by (auto simp: is_complete_def item_defs)
       qed
     qed
   qed
 qed
 
-lemma partially_completed_\<II>:
-  "wf_cfg cfg \<Longrightarrow> partially_completed (length inp) cfg inp (\<II> cfg inp) (\<lambda>_. True)"
-  by (simp add: \<II>_def partially_completed_\<I>)
-
-lemma Init_sub_\<I>:
-  "Init cfg \<subseteq> \<I> k cfg inp"
-  using \<pi>_mono by (induction k) (auto, blast, blast)
+lemma partially_completed_Earley:
+  "wf_cfg \<G> \<Longrightarrow> partially_completed (length \<omega>) \<G> \<omega> (Earley \<G> \<omega>) (\<lambda>_. True)"
+  by (simp add: partially_completed_Earley_k)
 
 lemma Derivation_\<SS>1:
-  assumes "Derivation cfg [\<SS> cfg] D inp" "is_word cfg inp" "wf_cfg cfg"
-  shows "\<exists>\<alpha> E. Derivation cfg \<alpha> E inp \<and> (\<SS> cfg,\<alpha>) \<in> set (\<RR> cfg)"
+  assumes "Derivation \<G> [\<SS> \<G>] D \<omega>" "is_word \<G> \<omega>" "wf_cfg \<G>"
+  shows "\<exists>\<alpha> E. Derivation \<G> \<alpha> E \<omega> \<and> (\<SS> \<G>,\<alpha>) \<in> set (\<RR> \<G>)"
 proof (cases D)
   case Nil
   thus ?thesis
     using assms is_nonterminal_startsymbol is_terminal_nonterminal by (metis Derivation.simps(1) is_word_def list.set_intros(1))
 next
   case (Cons d D)
-  then obtain \<alpha> where "Derives1 cfg [\<SS> cfg] (fst d) (snd d) \<alpha>" "Derivation cfg \<alpha> D inp"
+  then obtain \<alpha> where "Derives1 \<G> [\<SS> \<G>] (fst d) (snd d) \<alpha>" "Derivation \<G> \<alpha> D \<omega>"
     using assms by auto
-  hence "(\<SS> cfg, \<alpha>) \<in> set (\<RR> cfg)"
+  hence "(\<SS> \<G>, \<alpha>) \<in> set (\<RR> \<G>)"
     unfolding Derives1_def
     by (metis List.append.right_neutral List.list.discI append_eq_Cons_conv append_is_Nil_conv nth_Cons_0 self_append_conv2)
   thus ?thesis
-    using \<open>Derivation cfg \<alpha> D inp\<close> by auto
+    using \<open>Derivation \<G> \<alpha> D \<omega>\<close> by auto
 qed
 
 theorem completeness:
-  assumes "derives cfg [\<SS> cfg] inp" "is_word cfg inp" "wf_cfg cfg"
-  shows "earley_recognized (\<II> cfg inp) cfg inp"
+  assumes "derives \<G> [\<SS> \<G>] \<omega>" "is_word \<G> \<omega>" "wf_cfg \<G>"
+  shows "earley_recognized (Earley \<G> \<omega>) \<G> \<omega>"
 proof -
-  obtain \<alpha> where *: "(\<SS> cfg,\<alpha>) \<in> set (\<RR> cfg)" "derives cfg \<alpha> inp"
-    using Derivation_\<SS>1 assms Derivation_implies_derives derives_implies_Derivation by metis
-  let ?x = "Item (\<SS> cfg,\<alpha>) 0 0 0"
-  have "?x \<in> \<II> cfg inp" "wf_item cfg inp ?x"
-    unfolding \<II>_def using *(1) Init_sub_\<I> Init_def wf_Init by (auto simp: init_item_def, fast, fast)
-  moreover have "derives cfg (item_\<beta> ?x) inp"
-    using *(2) item_defs(4) by (simp add: item_\<beta>_def item_rule_body_def rule_body_def)
-  ultimately have "Item (\<SS> cfg,\<alpha>) (length \<alpha>) 0 (length inp) \<in> \<II> cfg inp"
-    using partially_completed_\<II> fully_completed wf_\<II> derives_implies_Derivation assms slice_id
-      slice_empty wf_item_def partially_completed_def
-    by (smt (verit, ccfv_SIG) item.sel(4) nat_le_linear)
+  obtain \<alpha> D where *: "(\<SS> \<G> ,\<alpha>) \<in> set (\<RR> \<G>)" "Derivation \<G> \<alpha> D \<omega>"
+    using Derivation_\<SS>1 assms derives_implies_Derivation by metis
+  define x where x_def: "x = Item (\<SS> \<G>, \<alpha>) 0 0 0"
+  have "partially_completed (length \<omega>) \<G> \<omega> (Earley \<G> \<omega>) (\<lambda>_. True)"
+    using assms(3) partially_completed_Earley by blast
+  hence 0: "partially_completed (length \<omega>) \<G> \<omega> (Earley \<G> \<omega>) (\<lambda>D'. length D' \<le> length D)"
+    unfolding partially_completed_def by blast
+  have 1: "x \<in> Earley \<G> \<omega>"
+    using x_def Earley.Init *(1) by fastforce
+  have 2: "Derivation \<G> (item_\<beta> x) D (slice 0 (length \<omega>) \<omega>)"
+    using *(2) x_def by (simp add: item_defs)
+  have "Item (\<SS> \<G>,\<alpha>) (length \<alpha>) 0 (length \<omega>) \<in> Earley \<G> \<omega>"
+    using partially_completed_upto[OF _ _ _ _ _ 2 0] wf_Earley 1 x_def by auto
   then show ?thesis
     unfolding earley_recognized_def is_finished_def by (auto simp: is_complete_def item_defs, force)
 qed
 
 subsection \<open>Correctness\<close>
 
-corollary correctness_set:
+corollary correctness:
   assumes "wf_cfg cfg" "is_word cfg inp"
-  shows "earley_recognized (\<II> cfg inp) cfg inp \<longleftrightarrow> derives cfg [\<SS> cfg] inp"
+  shows "earley_recognized (Earley cfg inp) cfg inp \<longleftrightarrow> derives cfg [\<SS> cfg] inp"
   using assms soundness completeness by blast
 
 
@@ -1142,8 +684,7 @@ lemma finiteness_UNIV_wf_item:
   using finiteness_empty finiteness_nonempty by fastforce
 
 theorem finiteness:
-  "finite (\<II> cfg inp)"
-  using finiteness_UNIV_wf_item wf_items_def wf_\<II> rev_finite_subset by (metis mem_Collect_eq subsetI)
-
+  "finite (Earley cfg inp)"
+  using finiteness_UNIV_wf_item wf_Earley rev_finite_subset by (metis mem_Collect_eq subsetI)
 
 end
